src/examples/Kuiper.Example.OnlineSoftmax.fst
@@ -8,8 +8,8 @@ open Kuiper.Tensor.Layout.Alg { l1_forward }
 
 module OSMX = Kuiper.Kernel.OnlineSoftmax
 
-let _test (len : szp) =
+let _test (len : szp{len <= max_blocks * max_threads}) =
   OSMX.online_softmax_gpu #f32 1024sz #len #(l1_forward len)
 
-let _testh (len : szp) =
+let _testh (len : szp{len <= max_blocks * max_threads}) =
   OSMX.online_softmax_gpu #f16 1024sz #len #(l1_forward len)
